src/CIU.v
@@ -1,62 +1,14 @@
-Require Import LogRel.
+Require Export Compatibility.
+
 Import ListNotations.
-
-(* Inductive Frame : Set :=
-| FApp1 (l : list Exp) (* apply □(e₁, e₂, ..., eₙ) *)
-| FApp2 (v : Exp) (p : is_value v) (l1 l2 : list Exp) (p2 : forall e, In e l2 -> is_value e) (** Can be problematic *)
-| FLet (v : Var) (e2 : Exp) (* let v = □ in e2 *)
-| FPlus1 (e2 : Exp) (* □ + e2 *)
-| FPlus2 (v : Exp) (p : is_value v) (* v + □ *)
-| FIf (e2 e3 : Exp) (* if □ then e2 else e3 *).
-
-Definition merge (F : Frame) (e : Exp) :=
-match F with
- | FApp1 l => 
- | FApp2 v p l1 l2 p2 => _
- | FLet v e2 => _
- | FPlus1 e2 => _
- | FPlus2 v p => _
- | FIf e2 e3 => _
-end
-
-
-Definition FrameStack := list Frame.
-
-Inductive Configuration : Type :=
-| ConfigReady (e : Exp)
-| ConfigStep (e : Exp) (F : FrameStack).
-
-Definition step (c : Configuration) : option Configuration :=
-match c with
-| ConfigReady e => None (* Should not be this ID? *)
-| ConfigStep e F =>
-  match e with
-  | ELit l =>
-    match F with
-    | [] => ConfigReady (ELit l)
-    | f::fs => ConfigStep (merge f (ELit l)) fs
-    end
-  | EVar v => _
-  | EFunId f => _
-  | EFun vl e => _
-  | ERecFun f vl e => _
-  | EApp exp l => _
-  | ELet v e1 e2 => _
-  | ELetRec f vl b e => _
-  | EPlus e1 e2 => _
-  | EIf e1 e2 e3 => _
-  end
-end. *)
-
 
 Definition CIU (e1 e2 : Exp) : Prop :=
   EXPCLOSED e1 /\ EXPCLOSED e2 /\
-  forall v1 clock,
-  eval clock e1 = Res v1 -> (exists v2, exists clock, eval clock e2 = Res v2 /\ equivalent_values v1 v2).
+  forall F, FCLOSED F -> | F, e1 | ↓ -> | F, e2 | ↓.
 
-Definition CIU_open (Γ : list VarFunId) (e1 e2 : Exp) :=
-  forall ξ, subscoped Γ [] ξ ->
-  CIU (subst ξ e1) (subst ξ e2).
+Definition CIU_open (Γ : nat) (e1 e2 : Exp) :=
+  forall ξ, SUBSCOPE Γ ⊢ ξ ∷ 0 ->
+  CIU (e1.[ξ]) (e2.[ξ]).
 
 Lemma CIU_closed :
   forall e1 e2,
@@ -74,7 +26,7 @@ Proof.
   intuition.
 Qed.
 
-Hint Resolve CIU_closed_l.
+Global Hint Resolve CIU_closed_l : core.
 
 Lemma CIU_closed_r : forall {e1 e2},
     CIU e1 e2 ->
@@ -85,7 +37,7 @@ Proof.
   intuition.
 Qed.
 
-Hint Resolve CIU_closed_r.
+Global Hint Resolve CIU_closed_r : core.
 
 Lemma CIU_open_scope : forall {Γ e1 e2},
     CIU_open Γ e1 e2 ->
@@ -94,7 +46,7 @@ Proof.
   intros.
   unfold CIU_open in H.
   split;
-    eapply sub_implies_scope_exp; eauto.
+    eapply subst_implies_scope_exp; eauto.
 Qed.
 
 Lemma CIU_open_scope_l : forall {Γ e1 e2},
@@ -106,7 +58,7 @@ Proof.
   intuition.
 Qed.
 
-Hint Resolve CIU_open_scope_l.
+Global Hint Resolve CIU_open_scope_l : core.
 
 Lemma CIU_open_scope_r : forall {Γ e1 e2},
     CIU_open Γ e1 e2 ->
@@ -118,7 +70,7 @@ Proof.
 Qed.
 
 
-Hint Resolve CIU_open_scope_r.
+Global Hint Resolve CIU_open_scope_r : core.
 
 Lemma Erel_implies_CIU : forall Γ e1 e2,
   Erel_open Γ e1 e2 ->
@@ -127,9 +79,10 @@ Proof.
   intros.
   unfold CIU_open; intros.
   unfold CIU.
-  split; [|split].
-  - eapply subst_preserves_scope_rev; eauto.
-  - eapply subst_preserves_scope_rev; eauto.
-  - intros. unfold Erel_open, Erel, exp_rel in H.
-    (* Vrel reflexivity needed *)
+  split. 2: split.
+  - apply -> (subst_preserves_scope_exp); eauto.
+  - apply -> (subst_preserves_scope_exp); eauto.
+  - unfold Erel_open, Erel, exp_rel in H. intros. destruct H2.
+    specialize (H x ξ ξ (Grel_Fundamental _ _ H0 _)). destruct H, H3.
+    eapply H4 in H2; eauto. apply Frel_Fundamental_closed. auto.
 Qed.
